md/src/references.md
@@ -14,6 +14,7 @@
 - G. Boolos, "The Logic of Provability"
 - M. C. Fitting, V. W. Marek, and M. Truszczynski, _"The Pure Logic of Necessitation"_
 - T. Kurahashi, _"The provability logic of all provability predicates"_
+- W. Carnielli, C. Pizzi, _"Modalities and Multimodalities"_
 
 ## Related Works
 
